intermediate/Veritas.Intermediate.Thread.fsti
@@ -132,3 +132,6 @@ val lemma_blum_evict_elem_prefix (#vcfg:_) (tl: verifiable_log vcfg) (i: nat{i <
 
 val lemma_add_clock (#vcfg:_) (tl: verifiable_log vcfg) (i: seq_index tl{is_blum_add (index tl i)}):
   Lemma (timestamp_of (blum_add_elem (index tl i)) `ts_lt`  clock tl i) 
+
+val lemma_evict_clock (#vcfg:_) (tl: verifiable_log vcfg) (i: seq_index tl{is_evict_to_blum (index tl i)}):
+  Lemma (timestamp_of (blum_evict_elem tl i) = clock tl i)
